Adding Hoare

trusted/Semantic.v
@@ -17,14 +17,16 @@ Inductive step : stmt -> data_state -> instr_state -> stmt -> data_state -> inst
     eval_expr env c = Bool true -> step st env ienv Skip env' ienv -> step (If c st sf) env ienv Skip env' ienv
 | step_if_false: forall env env' c st sf ienv,
     eval_expr env c = Bool false -> step sf env ienv Skip env' ienv -> step (If c st sf) env ienv Skip env' ienv
-| step_case: forall env env' z c se ls ienv,
-    eval_expr env c = Int z -> Z.le 0 z -> Some se = nth_error ls (Z.to_nat z) -> step se env ienv Skip env' ienv -> step (Case c ls) env ienv Skip env' ienv
+| step_case: forall env env' n c se ls ienv,
+    eval_expr env c = Int (Z.of_nat n) -> Some se = nth_error ls n -> step se env ienv Skip env' ienv -> step (Case c ls) env ienv Skip env' ienv
 | step_while_true: forall env env' env'' e s ienv,
     eval_expr env e = Bool true -> step s env ienv Skip env' ienv -> step (While e s) env' ienv Skip env'' ienv -> step (While e s) env ienv Skip env'' ienv
 | step_while_false: forall env e s ienv,
     eval_expr env e = Bool false -> step (While e s) env ienv Skip env ienv
 | step_call: forall env env' ienv fname,
     step (ienv fname) env ienv Skip env' ienv -> step (Call fname) env ienv Skip env' ienv
+| step_modify: forall (env: data_state) (ienv: instr_state) (a: string) (n e: expr) (i si ei: nat) (l: nat->DataTypes),
+    eval_expr env n = Int (Z.of_nat i) -> env a = Array (si, ei, l) -> si <= i -> i <= ei -> step (Modify a n e) env ienv Skip (update_state env a (Array (si, ei, update_array l i (eval_expr env e)))) ienv
 .
 
 
