trusted/Hoare.v
@@ -1,0 +1,83 @@
+Require Import Equality List ZArith.
+Require Import Syntax Semantic Evalexpr.
+
+Definition pred := data_state -> Prop.
+
+Definition valid_hoare_triple (senv: instr_state) (P: pred) (s: stmt) (Q: pred) : Prop :=
+    forall env1 env2, P env1 -> step s env1 senv Skip env2 senv -> Q env2.
+
+Theorem hoare_skip: forall senv P, valid_hoare_triple senv P Skip P.
+Proof.
+    unfold valid_hoare_triple. intros.
+    inversion H0. subst. apply H.
+Qed.
+
+Theorem hoare_assign:
+    forall senv P x e,
+    valid_hoare_triple senv (fun env => P (update_state env x (eval_expr env e))) (Assign x e) P.
+Proof.
+    unfold valid_hoare_triple. intros.
+    inversion H0. subst. apply H.
+Qed.
+
+Theorem hoare_comp:
+    forall senv P Q R s ls, valid_hoare_triple senv P s Q -> valid_hoare_triple senv Q (Seq ls) R
+    -> valid_hoare_triple senv P (Seq (s :: ls)) R.
+Proof.
+    unfold valid_hoare_triple. intros.
+    inversion H2. subst.
+    eapply H0. eapply H.
+    apply H1. apply H5. apply H8.
+Qed.
+
+Theorem hoare_seq_nil:
+    forall senv P, valid_hoare_triple senv P (Seq nil) P.
+Proof.
+    unfold valid_hoare_triple. intros.
+    inversion H0. subst. apply H.
+Qed.
+
+Theorem hoare_if:
+    forall senv c st sf P Q,
+    valid_hoare_triple senv (fun env => (eval_expr env c = Bool true) /\ P env) st Q ->
+    valid_hoare_triple senv (fun env => (eval_expr env c = Bool false) /\ P env) sf Q ->
+    valid_hoare_triple senv P (If c st sf) Q.
+Proof.
+    unfold valid_hoare_triple.
+    intros.
+    inversion H2 ; subst.
+    - eapply H. split. apply H8. apply H1. apply H11.
+    - eapply H0. split. apply H8. apply H1. apply H11.
+Qed.
+
+Theorem hoare_conseq:
+    forall senv P1 P2 s Q1 Q2,
+    (forall env, P1 env -> P2 env) -> valid_hoare_triple senv P2 s Q2 -> (forall env, Q2 env -> Q1 env) ->
+    valid_hoare_triple senv P1 s Q1.
+Proof.
+    unfold valid_hoare_triple. intros.
+    apply H1. eapply H0. apply H. apply H2. apply H3.
+Qed.
+
+Theorem hoare_while:
+    forall senv P e s,
+    valid_hoare_triple senv (fun env => (eval_expr env e = Bool true) /\ P env) s P -> 
+    valid_hoare_triple senv P (While e s) (fun env => (eval_expr env e) = Bool false /\ P env).
+Proof.
+    unfold valid_hoare_triple. intros.
+    dependent induction H1.
+    - eapply IHstep2 ; simpl ; intros ; auto.
+      + eapply H. apply H2. apply H3.
+      + eapply H. split. apply H1. apply H0. apply H1_.
+    - split. apply H1. apply H0.
+Qed.
+
+Theorem hoare_call:
+    forall fn P Q senv,
+    valid_hoare_triple senv P (senv fn) Q -> valid_hoare_triple senv P (Call fn) Q.
+Proof.
+    unfold valid_hoare_triple. intros.
+    inversion H1. subst.
+    eapply H. apply H0. apply H3.
+Qed.
+     
